CE_Equivs.v
@@ -1,0 +1,304 @@
+Require Export CE_FBOS.
+Require Export CE_NOS.
+
+Require Import Coq.Logic.FunctionalExtensionality.
+
+Axiom Expression_ind_2 :
+forall P : Expression -> Prop,
+       P ENil ->
+       (forall l : Literal, P (ELit l)) ->
+       (forall v : Var, P (EVar v)) ->
+       (forall f2 : FunctionIdentifier, P (EFunId f2)) ->
+       (forall (vl : list Var) (e : Expression), P e -> P (EFun vl e)) ->
+       (forall hd : Expression, P hd -> forall tl : Expression, P tl -> P (ECons hd tl)) ->
+       (forall l : list Expression, 
+         (forall i : nat, i < length l -> P (nth i l ENil)) ->
+       P (ETuple l)) ->
+       (forall (f6 : string) (l : list Expression), 
+         (forall i : nat, i < length l -> P (nth i l ENil)) ->
+       P (ECall f6 l)) ->
+       (forall exp : Expression, P exp -> 
+        forall l : list Expression,
+         (forall i : nat, i < length l -> P (nth i l ENil)) ->
+        P (EApp exp l)) ->
+       (forall e : Expression,
+        P e -> forall l : list (Pattern * Expression * Expression), 
+          (forall i : nat, i < length l -> P (snd (fst (nth i l (PNil, ENil, ENil))))) ->
+          (forall i : nat, i < length l -> P (snd (nth i l (PNil, ENil, ENil)))) ->
+        P (ECase e l)) ->
+       (forall (v : Var) (e1 : Expression),
+        P e1 -> forall e2 : Expression, P e2 -> P (ELet v e1 e2)) ->
+       (forall (f10 : FunctionIdentifier) (l : list Var) (b : Expression),
+        P b -> forall e : Expression, P e -> P (ELetRec f10 l b e)) ->
+       (forall e1 : Expression,
+        P e1 ->
+        forall (v1 : Var) (e2 : Expression),
+        P e2 -> forall (vl2 : list Var) (e3 : Expression), P e3 -> P (ETry e1 v1 e2 vl2 e3)) ->
+       forall e : Expression, P e.
+
+Theorem alma :
+forall l env id eff id' res eff' clock,
+(forall (env : Environment) (id : nat) (exp : Expression) 
+            (eff : SideEffectList) (id' : nat) (res : Value + Exception)
+            (eff' : SideEffectList),
+          eval_fbos_expr env id exp eff clock = Result id' res eff' ->
+          eval_fbos_expr env id exp eff (S clock) = Result id' res eff') ->
+(fix eval_list
+   (env : Environment) (id : nat) (exps : list Expression) 
+   (eff : SideEffectList) {struct exps} : ResultListType :=
+   match exps with
+   | nil => LResult id (inl nil) eff
+   | x :: xs =>
+       match eval_fbos_expr env id x eff clock with
+       | Result id' (inl v) eff' =>
+           match eval_list env id' xs eff' with
+           | LResult id'' (inl xs') eff'' => LResult id'' (inl (v :: xs')) eff''
+           | LResult id'' (inr _) _ => eval_list env id' xs eff'
+           | _ => eval_list env id' xs eff'
+           end
+       | Result id' (inr ex) eff' => LResult id' (inr ex) eff'
+       | Timeout => LTimeout
+       | Failure => LFailure
+       end
+   end) env id l eff = LResult id' res eff' ->
+(fix eval_list
+   (env : Environment) (id : nat) (exps : list Expression) 
+   (eff : SideEffectList) {struct exps} : ResultListType :=
+   match exps with
+   | nil => LResult id (inl nil) eff
+   | x :: xs =>
+       match eval_fbos_expr env id x eff clock with
+       | Result id' (inl v) eff' =>
+           match eval_list env id' xs eff' with
+           | LResult id'' (inl xs') eff'' => LResult id'' (inl (v :: xs')) eff''
+           | LResult id'' (inr _) _ => eval_list env id' xs eff'
+           | _ => eval_list env id' xs eff'
+           end
+       | Result id' (inr ex) eff' => LResult id' (inr ex) eff'
+       | Timeout => LTimeout
+       | Failure => LFailure
+       end
+   end) env id l eff =
+(fix eval_list
+   (env : Environment) (id : nat) (exps : list Expression) 
+   (eff : SideEffectList) {struct exps} : ResultListType :=
+   match exps with
+   | nil => LResult id (inl nil) eff
+   | x :: xs =>
+       match eval_fbos_expr env id x eff (S clock) with
+       | Result id' (inl v) eff' =>
+           match eval_list env id' xs eff' with
+           | LResult id'' (inl xs') eff'' => LResult id'' (inl (v :: xs')) eff''
+           | LResult id'' (inr _) _ => eval_list env id' xs eff'
+           | _ => eval_list env id' xs eff'
+           end
+       | Result id' (inr ex) eff' => LResult id' (inr ex) eff'
+       | Timeout => LTimeout
+       | Failure => LFailure
+       end
+   end) env id l eff.
+Proof.
+  induction l; intros.
+  * auto.
+  * case_eq (eval_fbos_expr env id a eff clock); intros.
+    - pose (H _ _ _ _ _ _ _ H1).
+      rewrite H1 in H0.
+      rewrite e. case_eq res0; intros; subst.
+      + (* pose (IHl env id0 eff0 id' res eff' clock H). *)
+        case_eq ((fix eval_list
+          (env : Environment) (id : nat) (exps : list Expression) 
+          (eff : SideEffectList) {struct exps} : ResultListType :=
+          match exps with
+          | nil => LResult id (inl nil) eff
+          | x :: xs =>
+              match eval_fbos_expr env id x eff clock with
+              | Result id' (inl v) eff' =>
+                  match eval_list env id' xs eff' with
+                  | LResult id'' (inl xs') eff'' => LResult id'' (inl (v :: xs')) eff''
+                  | LResult id'' (inr _) _ => eval_list env id' xs eff'
+                  | _ => eval_list env id' xs eff'
+                  end
+              | Result id' (inr ex) eff' => LResult id' (inr ex) eff'
+              | Timeout => LTimeout
+              | Failure => LFailure
+              end
+          end) env id0 l eff0); intros.
+       ** case_eq res0; intros.
+         -- inversion H0. subst.
+            pose (IHl env id0 eff0 id1 (inl l0) eff1 clock H H2).
+            rewrite <- e0. rewrite H2. auto.
+         -- inversion H0. subst.
+            pose (IHl env id0 eff0 id1 _ eff1 clock H H2).
+            rewrite <- e1. rewrite H2. auto.
+       ** rewrite H2 in H0. discriminate.
+       ** rewrite H2 in H0. discriminate.
+     + auto.
+   - rewrite H1 in H0. discriminate.
+   - rewrite H1 in H0. discriminate.
+Qed.
+
+Theorem clock_increase :
+  forall clock env id exp eff id' res eff',
+  eval_fbos_expr env id exp eff clock = Result id' res eff'
+->
+  eval_fbos_expr env id exp eff (S clock) = Result id' res eff'.
+Proof.
+  induction clock; intros; subst.
+  * simpl in H. inversion H.
+  * destruct exp.
+    - simpl in *. inversion H. auto.
+    - simpl in *. inversion H. auto.
+    - simpl in *. inversion H. auto.
+    - simpl in *. inversion H. auto.
+    - simpl in *. inversion H. auto.
+    - simpl in H. case_eq (eval_fbos_expr env id exp2 eff clock); intros.
+      + case_eq res0; intros; subst.
+        ** rewrite H0 in H. pose (IHclock _ _ _ _ _ _ _ H0).
+           case_eq (eval_fbos_expr env id0 exp1 eff0 clock); intros.
+           -- case_eq res0; intros; subst.
+             ++ rewrite H1 in H. pose (IHclock _ _ _ _ _ _ _ H1).
+                remember (S clock) as cl. simpl.
+                rewrite e. rewrite e0.
+                auto.
+             ++ rewrite H1 in H. pose (IHclock _ _ _ _ _ _ _ H1).
+                remember (S clock) as cl. simpl.
+                rewrite e. rewrite e1.
+                auto.
+          -- rewrite H1 in H. discriminate.
+          -- rewrite H1 in H. discriminate.
+        ** rewrite H0 in H. pose (IHclock _ _ _ _ _ _ _ H0).
+           remember (S clock) as cl. simpl. rewrite e0.
+           auto.
+      + rewrite H0 in H. discriminate.
+      + rewrite H0 in H. discriminate.
+    - simpl in H. 
+    remember ((fix eval_list
+          (env : Environment) (id : nat) (exps : list Expression) 
+          (eff : SideEffectList) {struct exps} : ResultListType :=
+          match exps with
+          | nil => LResult id (inl nil) eff
+          | x :: xs =>
+              match eval_fbos_expr env id x eff clock with
+              | Result id' (inl v) eff' =>
+                  match eval_list env id' xs eff' with
+                  | LResult id'' (inl xs') eff'' => LResult id'' (inl (v :: xs')) eff''
+                  | LResult id'' (inr _) _ => eval_list env id' xs eff'
+                  | _ => eval_list env id' xs eff'
+                  end
+              | Result id' (inr ex) eff' => LResult id' (inr ex) eff'
+              | Timeout => LTimeout
+              | Failure => LFailure
+              end
+          end) env id l eff) as result.
+    destruct result. 2-3: discriminate. symmetry in Heqresult.
+    assert ((fix eval_list
+               (env : Environment) (id : nat) (exps : list Expression) 
+               (eff : SideEffectList) {struct exps} : ResultListType :=
+               match exps with
+               | nil => LResult id (inl nil) eff
+               | x :: xs =>
+                   match eval_fbos_expr env id x eff clock with
+                   | Result id' (inl v) eff' =>
+                       match eval_list env id' xs eff' with
+                       | LResult id'' (inl xs') eff'' => LResult id'' (inl (v :: xs')) eff''
+                       | LResult id'' (inr _) _ => eval_list env id' xs eff'
+                       | _ => eval_list env id' xs eff'
+                       end
+                   | Result id' (inr ex) eff' => LResult id' (inr ex) eff'
+                   | Timeout => LTimeout
+                   | Failure => LFailure
+                   end
+               end) env id l eff = LResult id0 res0 eff0). { auto. }
+    pose (alma _ _ _ _ _ _ _ _ IHclock Heqresult). rewrite e in H0.
+    clear e. clear Heqresult.
+    remember (S clock) as cl. simpl. rewrite H0. assumption.
+    - simpl in H. 
+    remember ((fix eval_list
+          (env : Environment) (id : nat) (exps : list Expression) 
+          (eff : SideEffectList) {struct exps} : ResultListType :=
+          match exps with
+          | nil => LResult id (inl nil) eff
+          | x :: xs =>
+              match eval_fbos_expr env id x eff clock with
+              | Result id' (inl v) eff' =>
+                  match eval_list env id' xs eff' with
+                  | LResult id'' (inl xs') eff'' => LResult id'' (inl (v :: xs')) eff''
+                  | LResult id'' (inr _) _ => eval_list env id' xs eff'
+                  | _ => eval_list env id' xs eff'
+                  end
+              | Result id' (inr ex) eff' => LResult id' (inr ex) eff'
+              | Timeout => LTimeout
+              | Failure => LFailure
+              end
+          end) env id l eff) as result.
+    destruct result. 2-3: discriminate. symmetry in Heqresult.
+    assert ((fix eval_list
+               (env : Environment) (id : nat) (exps : list Expression) 
+               (eff : SideEffectList) {struct exps} : ResultListType :=
+               match exps with
+               | nil => LResult id (inl nil) eff
+               | x :: xs =>
+                   match eval_fbos_expr env id x eff clock with
+                   | Result id' (inl v) eff' =>
+                       match eval_list env id' xs eff' with
+                       | LResult id'' (inl xs') eff'' => LResult id'' (inl (v :: xs')) eff''
+                       | LResult id'' (inr _) _ => eval_list env id' xs eff'
+                       | _ => eval_list env id' xs eff'
+                       end
+                   | Result id' (inr ex) eff' => LResult id' (inr ex) eff'
+                   | Timeout => LTimeout
+                   | Failure => LFailure
+                   end
+               end) env id l eff = LResult id0 res0 eff0). { auto. }
+    pose (alma _ _ _ _ _ _ _ _ IHclock Heqresult). rewrite e in H0.
+    clear e. clear Heqresult.
+    remember (S clock) as cl. simpl. rewrite H0. assumption.
+Admitted.
+
+Theorem bigger_clock :
+  forall clock clock' env id exp eff id' res eff',
+  clock < clock' ->
+  eval_fbos_expr env id exp eff clock = Result id' res eff'
+->
+  eval_fbos_expr env id exp eff clock' = Result id' res eff'.
+Proof.
+  intros. induction H.
+  * apply clock_increase. auto.
+  * apply clock_increase. auto.
+Qed.
+
+Theorem nos_equiv_fbos :
+  forall env id exp eff id' res eff',
+  | env, id, exp, eff | -e> |id', res, eff'|
+->
+  (exists clock, eval_fbos_expr env id exp eff clock = Result id' res eff').
+Proof.
+  intro. intro. intro. generalize dependent id. induction exp using Expression_ind_2; intros.
+  1-5: exists 1; simpl; inversion H; auto; rewrite H3; auto.
+  * inversion H; subst.
+    - pose (IHexp2 _ _ _ _ _ H4).
+      pose (IHexp1 _ _ _ _ _ H9).
+      inversion e. inversion e0.
+      exists (S (x + x0)). simpl. admit.
+    - admit.
+    - admit.
+  * inversion H0. subst.
+    exists (S ?[r]).
+
+
+
+
+
+
+
+
+
+
+
+
+
+
+
+
+
+
